---
created: 2025-03-30 13:19:12
modified: 2025-03-30 13:19:17
title: Untitled
---
# Untitled

I'll help you prove that $|\alpha\beta| = |\alpha| + |\beta|$ for any strings $\alpha$ and $\beta$ over an alphabet $\Sigma$.

First, let me note that there appears to be a small typo in your inductive case definition. It should probably be $|\alpha| = 1 + |\gamma|$ rather than $|\alpha| = 1|\gamma|$.

Let's proceed with the proof by induction on the length of $\beta$.

**Base Case**: $\beta = \lambda$ (the empty string)

When $\beta = \lambda$, we have:

$|\alpha\beta| = |\alpha\lambda| = |\alpha|$ (since concatenating with the empty string doesn't change the string)

Also, $|\alpha| + |\beta| = |\alpha| + |\lambda| = |\alpha| + 0 = |\alpha|$

Therefore, $|\alpha\beta| = |\alpha| + |\beta|$ holds for the base case.

**Inductive Hypothesis**: Assume that for some string $\beta$, the property $|\alpha\beta| = |\alpha| + |\beta|$ holds for all strings $\alpha$.

**Inductive Step**: We need to prove that $|\alpha\beta b| = |\alpha| + |\beta b|$ for any $b \in \Sigma$.

Let's work through this:

1. $|\alpha\beta b| = |(\alpha\beta)b|$
2. By the inductive definition of length (case b), $|(\alpha\beta)b| = 1 + |\alpha\beta|$
3. By the inductive hypothesis, $|\alpha\beta| = |\alpha| + |\beta|$
4. Substituting, $|(\alpha\beta)b| = 1 + |\alpha| + |\beta|$
5. By the inductive definition of length, $|\beta b| = 1 + |\beta|$
6. Therefore, $|\alpha| + |\beta b| = |\alpha| + (1 + |\beta|) = |\alpha| + 1 + |\beta| = 1 + |\alpha| + |\beta|$
7. From steps 4 and 6, we have $|\alpha\beta b| = |\alpha| + |\beta b|$

This completes the induction, proving that $|\alpha\beta| = |\alpha| + |\beta|$ for all strings $\alpha$ and $\beta$ over the alphabet $\Sigma$.
